Splinter/Betree/LinkedBranch.i.dfy
@@ -32,6 +32,7 @@ module LinkedBranchMod {
   datatype TransitionLabel = 
     | QueryLabel(key: Key, msg: Message)
     | InsertLabel(key: Key, msg: Message)
+    | AppendLabel(keys: seq<Key>, msgs: seq<Message>) // insert into a new leaf
     | InternalLabel(addr: Address)
 
   datatype Node = Index(pivots: seq<Key>, children: seq<Address>) | Leaf(keys: seq<Key>, msgs: seq<Message>)
@@ -374,6 +375,19 @@ module LinkedBranchMod {
       LinkedBranch(root, diskView.ModifyDisk(root, newNode))
     }
 
+    // Append
+    function AppendToNewLeaf(newKeys: seq<Key>, newMsgs: seq<Message>) : (result: LinkedBranch)
+    requires WF()
+    requires Root().Leaf?
+    requires |newKeys| == |newMsgs|
+    requires Keys.IsStrictlySorted(newKeys)
+    ensures result.WF()
+    {
+      var newNode := Leaf(newKeys, newMsgs);
+      var newDiskView := diskView.ModifyDisk(root, newNode);
+      LinkedBranch(root, newDiskView)
+    }
+
     // Split
 
     predicate SplitLeaf(pivot: Key, leftLeaf: LinkedBranch, rightLeaf: LinkedBranch)
@@ -495,6 +509,14 @@ module LinkedBranchMod {
     {
       LinkedBranch(branch.root, replacement.diskView)
     }
+
+    predicate PathEquiv(otherKey: Key)
+      requires Valid()
+      decreases depth, 1
+    {
+      && branch.Root().Route(key) == branch.Root().Route(otherKey)
+      && (0 < depth ==> Subpath().PathEquiv(otherKey))
+    }
   }
 
   datatype Variables = Variables(branch: LinkedBranch)
@@ -517,8 +539,27 @@ module LinkedBranchMod {
     && lbl.InsertLabel?
     && v.WF()
     && path.Valid()
+    && path.branch == v.branch
+    && path.key == lbl.key
     && path.Target().Root().Leaf?
     && newTarget == path.Target().InsertLeaf(lbl.key, lbl.msg)
+    && v'.branch == path.Substitute(newTarget)
+  }
+
+  predicate Append(v: Variables, v': Variables, lbl: TransitionLabel, path: Path, newTarget: LinkedBranch)
+  {
+    && lbl.AppendLabel?
+    && v.WF()
+    && path.Valid()
+    && path.branch == v.branch
+    && path.Target().Root() == Leaf([], [])
+    && lbl.keys != []
+    && |lbl.keys| == |lbl.msgs|
+    && Keys.IsStrictlySorted(lbl.keys)
+
+    && newTarget == path.Target().AppendToNewLeaf(lbl.keys, lbl.msgs)
+    && path.key == newTarget.Root().keys[0]
+    && path.PathEquiv(Last(newTarget.Root().keys))
     && v'.branch == path.Substitute(newTarget)
   }
 
@@ -536,8 +577,8 @@ module LinkedBranchMod {
     && lbl.InternalLabel?
     && v.WF()
     && path.Valid()
+    && path.branch == v.branch
     && v.branch.diskView.IsFresh({lbl.addr})
-    && path.branch.root == v.branch.root
     && path.Target().SplitChildOfIndex(pivot, lbl.addr, newTarget)
     && v'.branch == path.Substitute(newTarget)
   }
@@ -552,6 +593,7 @@ module LinkedBranchMod {
   datatype Step =
     | QueryStep()
     | InsertStep(path: Path, newTarget: LinkedBranch)
+    | AppendStep(path: Path, newTarget: LinkedBranch)
     | GrowStep()
     | SplitStep(path: Path, pivot: Key, newTarget: LinkedBranch)
 
@@ -560,6 +602,7 @@ module LinkedBranchMod {
     match step {
       case QueryStep() => Query(v, v', lbl)
       case InsertStep(path, newTarget) => Insert(v, v', lbl, path, newTarget)
+      case AppendStep(path, newTarget) => Append(v, v', lbl, path, newTarget)
       case GrowStep() => Grow(v, v', lbl)
       case SplitStep(path, pivot, newTarget) => Split(v, v', lbl, path, pivot, newTarget)
     }
